Wasm/Compiler.lean
@@ -1,0 +1,128 @@
+import Wasm
+
+inductive Expr : ValType -> Type
+| I32Lit (n : UInt32) : Expr .I32
+| F32Lit (n : Float) : Expr .F32
+| I32Add (lhs : Expr .I32) (rhs : Expr .I32) : Expr .I32
+| I32Sub (lhs : Expr .I32) (rhs : Expr .I32) : Expr .I32
+| F32Add (lhs : Expr .F32) (rhs : Expr .F32) : Expr .F32
+
+def Expr.eval (e : Expr T) : T.repr := match e with
+| .I32Lit n => n
+| .F32Lit n => n
+| .I32Add lhs rhs => lhs.eval + rhs.eval
+| .I32Sub lhs rhs => lhs.eval - rhs.eval
+| .F32Add lhs rhs => lhs.eval + rhs.eval
+
+def testExpr : Expr .I32 := .I32Add (.I32Lit 5) (.I32Add (.I32Lit 10) (.I32Lit 15))
+def evalRes := testExpr.eval
+#eval evalRes
+
+def Expr.compile (e : Expr T) : Prog inp (T::inp) := match e with
+| .I32Lit n => Prog.cons (.I32Const n) (Prog.nil)
+| .F32Lit n => Prog.cons (.F32Const n) (Prog.nil)
+| .I32Add lhs rhs => (Prog.concat lhs.compile rhs.compile).append (.I32Add)
+| .I32Sub lhs rhs => (Prog.concat lhs.compile rhs.compile).append (.I32Sub)
+| .F32Add lhs rhs => (Prog.concat lhs.compile rhs.compile).append (.F32Add)
+
+def compiledExpr (inp : StackTypes := []) : Prog inp (.I32::inp) := testExpr.compile
+def compileRes := evalProg [] compiledExpr
+#eval compileRes
+
+def progResHead (progRes : { result : Stack // result.types = (x::xs) }) : { val : Val // val.toValType = x } :=
+  let ⟨st, h⟩ := progRes
+  let hd::tl := st
+  have h' : hd.toValType = x := by
+    unfold Stack.types at h;
+    rw [List.map_cons, List.cons_eq_cons] at h; apply h.left;
+  ⟨hd, h'⟩
+
+def eval_eq_compile (e : Expr T) : Prop :=
+  let prog := @e.compile T []
+  let compile_res := evalProg [] prog
+  let ⟨res, h⟩ := progResHead compile_res
+  let eval_res := e.eval
+  have h' : T.repr = res.toValType.repr := by rw [h]
+  res.toRepr = (h' ▸ eval_res)
+
+def test_expr_eq : Bool :=
+  let prog := testExpr.compile
+  let compile_res := evalProg [] prog
+  let ⟨res, h⟩ := progResHead compile_res
+  have h' : UInt32 = res.toValType.repr := by rw [h]
+  let res : UInt32 := (h' ▸ res.toRepr)
+  let eval_res := testExpr.eval
+  res == eval_res
+#eval test_expr_eq
+
+@[simp]
+theorem eval_nil {st : Stack} {h : st.types = inpTys} : (evalProg' (@Prog.nil inpTys) st h).val = st := by
+  unfold evalProg'; rfl
+
+/- @[simp] -/
+/- theorem prog_cast_nil {a b : StackTypes} (h : a = b) : (h ▸ (@Prog.nil a)) = (@Prog.nil b) := by -/
+/-   subst h; rfl -/
+
+@[simp]
+theorem concat_nil {a b : StackTypes} {lhs : Prog a b} : Prog.concat lhs Prog.nil = lhs := by
+  induction lhs with
+  | nil => rfl
+  | cons op rest ih => unfold Prog.concat; rw [ih];
+
+theorem concat_eval {a b c : StackTypes} 
+  (left : Prog a b) (right : Prog b c) 
+  (astack : Stack) (ah : astack.types = a)
+  :
+    let ⟨bstack, bh⟩ := evalProg' left astack ah
+    evalProg' (Prog.concat left right) astack ah = evalProg' right bstack bh
+:= by
+  dsimp;
+  induction right with
+  | nil => aesop
+  | cons r_op rrest r_ih => sorry
+  /- induction left with -/
+  /- | @nil s => -/
+  /-     conv => rhs; arg 2; rw [eval_nil]; -/
+  /-     unfold Prog.concat; -/ 
+  /-     rfl -/
+  /- | cons l_op lrest l_ih => -/
+  /-     have : -/ 
+      /- induction right with -/
+      /- | @nil s => rw [concat_nil]; rfl -/
+      /- | cons r_op rrest r_ih => -/
+      /-     conv => rhs; -/ 
+
+          
+
+        
+  /- obtain ⟨bstack, bh⟩ := (evalProg astack (ah ▸ left)) -/
+  /- show _ = _; -/
+  /- induction h : left generalizing astack with -/
+  /- | @nil s => -/ 
+
+  /-     sorry -/
+
+theorem compile_head_eq_eval : ∀ (e : Expr T), eval_eq_compile e := by
+  intro e; unfold eval_eq_compile; intro prog compile_res; simp;
+  induction e with
+  | I32Lit n =>
+      unfold progResHead;
+      have hc : compile_res = ⟨[Val.I32 n], by simp⟩ := by
+        (unfold compile_res; unfold prog Expr.compile evalProg evalOp evalProg; dsimp)
+      rw [hc]; dsimp; rfl;
+  | F32Lit n =>
+      unfold progResHead;
+      have hc : compile_res = ⟨[Val.F32 n], by simp⟩ := by
+        (unfold compile_res; unfold prog Expr.compile evalProg evalOp evalProg; dsimp)
+      rw [hc]; dsimp;
+      unfold Expr.eval; rfl;
+  | I32Add lhs rhs lhs_ih rhs_ih =>
+      unfold progResHead compile_res;
+      have hc : compile_res = sorry := by (
+        unfold compile_res prog Expr.compile;
+        have : evalProg [] (Prog.concat lhs.compile rhs.compile) = sorry := by (
+          unfold Prog.concat; dsimp; sorry)
+  /- have ⟨res, h⟩ := progResHead compile_res; -/
+  /- have h' : T.repr = res.toValType.repr := by rw [h]; -/
+  /- show (res.toRepr = h' ▸ e.eval); -/
+  /- induction e with -/
